TypeSubstの補題を追加

theorems/TypeSubst.v
@@ -31,6 +31,189 @@ Fixpoint term_subst t tsubst :=
      If (term_subst t1 tsubst) (term_subst t2 tsubst) (term_subst t3 tsubst)
   end.
 
+Definition union {A : Type} (tsubst1 tsubst2 : table A) :=
+  Table.fold (fun key e m => Table.add key e m) tsubst1 tsubst2.
+
+Definition filter {A : Type} {P : string -> Prop} (dec : forall x, {P x} + {~ P x}) (tsubst : table A) :=
+  TableProp.filter
+    (fun key _ => if dec key then true else false)
+    tsubst.
+
+Lemma mapsto_type_subst: forall x tsubst1 tsubst2,
+ (forall U,Table.MapsTo x U tsubst1 <-> Table.MapsTo x U tsubst2) ->
+ type_subst (VarT x) tsubst1 = type_subst (VarT x) tsubst2.
+Proof.
+intros.
+simpl in |- *.
+destruct (TableWF.In_dec tsubst1 x).
+ unfold Table.In in i.
+ unfold Table.Raw.PX.In in i.
+ decompose [ex] i.
+ generalize H0.
+ intro.
+ apply H in H1.
+ apply TableWF.find_mapsto_iff in H0.
+ apply TableWF.find_mapsto_iff in H1.
+ rewrite H0 in |- *; rewrite H1 in |- *.
+ reflexivity.
+
+ assert (~ Table.In (elt:=type) x tsubst2).
+  intro; apply n.
+  unfold Table.In in H0.
+  unfold Table.Raw.PX.In in H0.
+  decompose [ex] H0.
+  unfold Table.In in |- *.
+  unfold Table.Raw.PX.In in |- *.
+  exists x0.
+  apply <- H (* Generic printer *).
+  trivial.
+
+  apply TableWF.not_find_mapsto_iff in n.
+  apply TableWF.not_find_mapsto_iff in H0.
+  rewrite n in |- *; rewrite H0 in |- *.
+  reflexivity.
+Qed.
+
+Lemma union_iff: forall A x (T : A) (X Y : table A),
+  Table.MapsTo x T (union X Y) <-> Table.MapsTo x T X \/ (~ Table.In x X /\ Table.MapsTo x T Y).
+Proof.
+intros.
+unfold union in |- *.
+pattern X,
+ (Table.fold
+    (fun (key : Table.key) (e : A) (m : Table.t A) => Table.add key e m) X Y)
+ in |- *.
+apply TableProp.fold_rec_bis; intros.
+ apply Extensionality_Table in H.
+ rewrite <- H in |- *.
+ trivial.
+
+ split; intros.
+  right.
+  split.
+   intro.
+   apply TableWF.empty_in_iff in H0.
+   contradiction .
+
+   trivial.
+
+  decompose [or] H.
+   inversion H0.
+
+   decompose [and] H0.
+   trivial.
+
+ split; intros.
+  apply TableWF.add_mapsto_iff in H2.
+  decompose [or] H2.
+   left.
+   decompose [and] H3.
+   rewrite H4 in |- *; rewrite H5 in |- *.
+   apply <- TableWF.add_mapsto_iff (* Generic printer *).
+   left; split; reflexivity.
+
+   decompose [and] H3.
+   apply H1 in H5.
+   decompose [or] H5.
+    left.
+    apply <- TableWF.add_mapsto_iff (* Generic printer *).
+    right.
+    split; trivial.
+
+    decompose [and] H6.
+    right.
+    split.
+     intro.
+     apply H7.
+     apply TableWF.add_in_iff in H9.
+     decompose [or] H9.
+      contradiction .
+
+      trivial.
+
+     trivial.
+
+  decompose [or] H2.
+   apply TableWF.add_mapsto_iff in H3.
+   decompose [or] H3.
+    decompose [and] H4.
+    rewrite H5 in |- *; rewrite H6 in |- *.
+    apply <- TableWF.add_mapsto_iff (* Generic printer *).
+    left.
+    split; reflexivity.
+
+    decompose [and] H4.
+    apply <- TableWF.add_mapsto_iff (* Generic printer *).
+    right.
+    split.
+     trivial.
+
+     apply H1.
+     left.
+     trivial.
+
+   decompose [and] H3.
+   apply <- TableWF.add_mapsto_iff (* Generic printer *).
+   right.
+   split.
+    intro.
+    apply H4.
+    apply <- TableWF.add_in_iff (* Generic printer *).
+    left.
+    trivial.
+
+    apply H1.
+    right.
+    split.
+     intro.
+     apply H4.
+     apply <- TableWF.add_in_iff (* Generic printer *).
+     right.
+     trivial.
+
+     trivial.
+Qed.
+
+Lemma filter_iff : forall A x P (dec : forall x, {P x} + {~ P x}) (T : A) (m : table A),
+  Table.MapsTo x T (filter dec m) <-> Table.MapsTo x T m /\ (P x).
+Proof.
+unfold filter in |- *.
+intros; split; intros.
+ apply TableProp.filter_iff in H.
+  intro.
+  unfold Morphisms.respectful in |- *.
+  intros.
+  rewrite H0 in |- *.
+  reflexivity.
+
+  decompose [and] H.
+  split.
+   trivial.
+
+   destruct (dec x).
+    trivial.
+
+    discriminate.
+
+ apply <- TableProp.filter_iff (* Generic printer *).
+  decompose [and] H.
+  split.
+   trivial.
+
+   destruct (dec x).
+    reflexivity.
+
+    contradiction .
+
+  unfold Morphisms.Morphism in |- *.
+  unfold Morphisms.respectful in |- *.
+  intros.
+  rewrite H0 in |- *.
+  reflexivity.
+Qed.
+
+
+
 (*Lemma add_eq : forall x T tenv tsubst,
   (Table.add x (type_subst T tsubst) (tenv_subst tenv tsubst)) = (tenv_subst (Table.add x T tenv) tsubst).
 Proof.
